Cleaning up propositional logic files

dafny/propositional-logic/consequence.dfy
@@ -4,9 +4,19 @@ module consequence
 {
     import opened syntax
     import opened interpretation
-    import opened semantics
+    import opened evaluation
     import opened model
     import opened decision
+
+    /*
+    In the area of logical reasoning, the term "context" is generally
+    used to refer to a set of propositions that is taken as true for the
+    purposes of reasoning about the truth of a follow-on proposition.
+    The goal is generally to show that "in the context of a set of zero
+    or more assumptions (the "context") some conclusion must be true."
+    We represent a context as a sequence of propositions, and give this
+    type the name/synonmy pContext. 
+    */
 
     type pContext = seq<pExp>
 
@@ -21,10 +31,17 @@ module consequence
     /*
     Given a list of propositions, return their conjunction. E.g.,
     given [P1, P2, P3], return pAnd(P1(pAnd(P2,(pAnd(P3, pTrue))).
-    To terminate the recursion, we throw in that extra pTrue as
-    a last proposition in the resulting nested expression.
+    Note that the recursion ends with the empty list of premises
+    being equated to pTrue. pTrue is the "identity element" when it 
+    comes to *evaluating* a conjunction of other propositions, so it
+    is the right value to use in that sense. And if the whole list 
+    of premises really was empty (not just at the end of a recursion),
+    it is still the right value, in that the resulting implication 
+    would just say, "In any case at all, not conditioned on any other
+    propositions being true, the conclusion is true." 
     */
-    function method conjoinPremises(premises: seq<pExp>): pExp{
+    function method conjoinPremises(premises: seq<pExp>): pExp
+    {
         if |premises|==0 then pTrue
         else pAnd(premises[0], conjoinPremises(premises[1..]))
     }
