dafny/propositional-logic/evaluation.dfy
@@ -1,28 +1,23 @@
  include "interpretation.dfy"
  
- module semantics
+ module evaluation
  {
      import opened syntax
      import opened interpretation
 
     /*
-    Evaluate a propositional expression given an interpretation.
-    The recursive structure of this algorithm again reflects the
-    inductive structure of the expressions defined by the syntax
-    of our language.
+    Evaluate a propositional expression given an interpretation,
+    yielding a Dafny Boolean values as a result. The recursive 
+    structure of this code mirrors the inductive definition of 
+    the syntax of expressions in propositional logic. 
     */
     function method pEval(e: pExp, i: pInterpretation): (r: bool)
     {
         match e 
         {
-            // Evaluate constants (literals) to corresponding values
             case pTrue => true
             case pFalse => false
-
-            // Evaluate variable expressions by lookup in environment
             case pVarExp(v: pVar) => pVarValue(v,i)
-
-            // Evaluate operator exprs recursively in same environment
             case pNot(e1: pExp) => !pEval(e1,i)
             case pAnd(e1, e2) => pEval(e1,i) && pEval(e2, i)
             case pOr(e1, e2) =>  pEval(e1, i) || pEval(e2, i)
