dafny/propositional-logic/interpretation.dfy
@@ -5,156 +5,78 @@
     import opened syntax
 
    /*
-    We define an "interpretation" that maps our
-    Boolean variables to corresponding (bool) values. 
-    In programming languages, such a mapping from
-    variables to values is called an environment. 
-    Another term for the same idea is "state." The
-    state of a program is the value of each of its
-    variables at a given point in program execution.
-    
-    We represent an interpretation as a Dafny map
-    from our own Boolean variables to Dafny bool 
-    values: i.e., map<bVar,bool>. 
+    An "interpretation" maps propositional variables
+    to Boolean values. We represent an interpretation 
+    as a Dafny map from pVar values to to Dafny bools:
+    i.e., map<bVar,bool>. 
     
     When we need to evaluate a variable expression, 
     we'll  look up the value of the variable in such
     a map. 
 
-    To make the purpose of this particular type of
-    map clear, we define a "type synonym," namely 
-    "pInterpretation." From this point on, instead 
-    of writing map<bVar, bool> we use the synonym.
-    Type synonyms don't change the behavior of code
-    in any way, but they can make the intent of the 
-    code clearer to human readers. In this sense,
-    they support a form of "abstraction", hiding 
-    complex details behind a more meaningful name.
+    We define a "type synonym," pInterpretation, for 
+    map<bVar,bool>. Type synonyms don't change the 
+    behavior of code. Rather, they serve to document 
+    the purpose of the code for human readers. In this 
+    sense, they support a form of "abstraction", hiding 
+    complex details behind a simpler, meaningful name.
     */
 
     type pInterpretation = map<pVar, bool>
 
+ 
     /*
-    We note that a map might not be "total": that
-    is, it might not contain an entry for every 
-    variable (bVar) we have declared to exist. If
-    we try to look up a value that is not defined
-    in the map, we'll get an error. For example, if
-    i is an interpetation (a map<string, bool>) and
-    we try to look up the bool value for a string
-    that isn't defined in the map, e.g., "FooBar",
-    it won't work.
-
-    Our solution for now will be to define a function
-    that takes an interpretation and a string to look
-    up and that returns the value for the string in the
-    map if it's defined in the map, and that returns
-    the value "false" as a default if the string is 
-    not in the map. 
-    
-    This isn't a great design, in that a return of 
-    "false" could mean one of two things: either the 
-    value of the variable really is false, or it's 
-    just not assigned a value in the interpretation. 
-    For now, our design is good enough to illustate 
-    our main points.
+    This method returns the value assigned to a given
+    propositional variable by a given interpretation,
+    or false if the variable's not mapped by it. The
+    design of this code would be improved by the
+    addition of a precondition that requires v in i.
     */
-
     function method pVarValue(v: pVar, i: pInterpretation): bool
-        //    requires v in i
     {
-        //    i[v]
         if (v in i) then i[v] else false
     }
 
-    method show_pInterps(interps: seq<pInterpretation>, vs: seq<pVar>)
-    {
-        var i := 0;
-        print "{\n";
-        while (i < |interps|)
-        {
-            show_pInterp(vs, interps[i]);
-            if i < |interps| - 1 { print ",\n"; }
-            i := i + 1;
-        }
-        print "\n}\n";
-    }
 
-    method show_pInterp(vs: seq<pVar>, interp: pInterpretation)
-        //requires forall v :: v in vs ==> v in interp
+    /*
+    This method serializes an interpretation to a string,
+    using the string name of each variable in the output.
+    The design would be improved by a pre-condition that
+    requires forall v :: v in vs ==> v in interp.
+    */
+    method show_pInterp(interp: pInterpretation, vs: seq<pVar>)
     {
         var n := | vs |;
         var i := 0;
         print "[";
         while (i < n) {
-            match vs[i] 
+            if vs[i] in interp 
             {
-                case mkPVar(s:string) => 
-                    if vs[i] in interp {
-                        print s, " := ", interp[vs[i]], ", ";
-                    }
+                print vs[i].name, " := ", interp[vs[i]], ", ";
             }
             i := i + 1;
         }
         print "]";
     }
-
-    /*
-    Given a sequence, vs, of Boolean variables, return a 
-    sequence of all (2^|vs|) possible interpretations, i.e.,
-    mappings from these variables to Boolean values. Watch
-    out: for large numbers of variables the result be very
-    large.
-    */
+ 
+ /*
+ This method serializes a sequence of interpretations,
+ using the preceding method to serialize each one, and 
+ is mainly used to output, for example, lists of models 
+ or counterexamples of given propositions.
+ */
+ method show_pInterps(interps: seq<pInterpretation>, vs: seq<pVar>)
+    {
+        var i := 0;
+        print "{\n";
+        while (i < |interps|)
+        {
+            show_pInterp(interps[i], vs);
+            if i < |interps| - 1 { print ",\n"; }
+            i := i + 1;
+        }
+        print "\n}\n";
+    }
  }
 
-    /*************** 
-
-    function method init_interp'(vs: seq<pVar>): pInterpretation
-    {
-        init_interp'_helper(vs, map[])
-    }
-
-
-
-    function method init_interp'_helper(vs: seq<pVar>, i: pInterpretation): (p: pInterpretation)
-        // ensures forall v :: v in vs ==> v in p
-    {
-        if | vs | == 0 
-        then i
-        else init_interp'_helper(vs[1..], i[vs[0] := false])
-    }
-
-
-    function method next_interp'(vs: seq<pVar>, a: seq<pInterpretation>): pInterpretation
-        requires | a | >= 1;
-    {
-        increment_interp'(vs, a[0], | vs |)
-    }
-
-
-    function method  increment_interp' (vs: seq<pVar>, i: pInterpretation, idx: nat): pInterpretation
-        requires 0 <= idx < |vs|
-        requires forall v :: v in vs ==> v in i
-    {
-       if idx == 0 then i 
-       else if vs[idx] !in i then i
-       else if i[vs[idx]] == false then i[ vs[idx] := true ]
-       else increment_interp'(vs, i[ vs[idx] := false ], idx - 1)
-    }
-
-    function method all_interps'(vs: seq<pVar>): (result: seq<pInterpretation>)
-    {
-        all_interps'_help(vs, pow2(|vs|), [ init_interp'(vs) ])
-    }
-
-    function method all_interps'_help(vs: seq<pVar>, fl: nat, a: seq<pInterpretation>):
-        (result: seq<pInterpretation>)
-            requires | a |  >= 1;
-    {
-        if fl == 0 
-        then a  
-        else all_interps'_help(vs, fl - 1, [ next_interp'(vs, a)] + a )     
-    }
-}
-    */
+ 
