dafny/propositional-logic/truth_table.dfy
@@ -1,8 +1,9 @@
 include "interpretation.dfy"
-
+include "variables.dfy"
 module truth_table
 {
     import opened syntax
+    import opened variables
     import opened interpretation
 
     /*
@@ -10,28 +11,18 @@ module truth_table
     interpretations for a given sequence of Boolean
     variables, in increasing order from all false to
     all true. Each interpretation is a map from each
-    of the variables to that variable's value under
-    the given interpretation. In other words, this
-    method returns the "input" parts of each row of 
-    a truth table for the given sequence of Boolean
-    variables. We'll introduce a type synonym to
-    express this abstraction. 
+    of the variables to that variable's bool value 
+    under the given interpretation. In other words, 
+    this method returns the "input" parts of each row 
+    of a truth table for the given propositional
+    variables. 
     */
-
-    type truthTableInputs = seq<pInterpretation>
-    // plus constraint that all combinations are represented
-
-    /*
-    A currently unverified precondition is that no
-    variable may occur in "vs" more than once.
-    */
-    method all_interps(e: pExp) 
-        returns (result: truthTableInputs)
-        // requires forall v :: | (toBag(vs))[v] <= 1 |
+    method truth_table_inputs(e: pExp) 
+        returns (result: seq<pInterpretation>)
     {
-        var vs: seq<pVar> := seqVarsIn(e);
+        var vs := seqVarsIn(e);
         result := [];
-        var interp := all_false_interp(e);
+        var interp := all_false_interp(vs);
         var i: nat := 0;
         var n := pow2(|vs|);
         while (i < n)
@@ -48,33 +39,27 @@ module truth_table
         the sequence vs such that every variable maps 
         to false.
     */
-    method all_false_interp(e: pExp) 
+    method all_false_interp(vs: seq<pVar>) 
         returns (result: pInterpretation)
     {
-        var vs := seqVarsIn(e);
-    
-        // start with an empty map
         result := map[];
-
-        // iterate through variables in vs
         var i := 0;
         while (i < | vs |)
         {
-            // for each one, add a maplet from it to false
             result := result[ vs[i] := false ];
             i := i + 1;
         }
 
-        // that's it
         return result;
     }
 
     /*
-    Takes a sequence of variables and an interpretation
-    (meant to be) for those variables, and computes the
-    "next" interpretation for those variables. It does this
-    by in effect treating the sequence of values as a 
-    binary integer and by incrementing it by one.
+    Given a sequence of variables and an interpretation
+    for those variables, computes a "next" interpretation.
+    Treat the sequence of values as a binary integer and 
+    increment it by one. Any variables in vs that are not
+    in interp are ignored. Would be better to enforce a
+    pre-condition to rule out this possibility.
     */
     method next_interp(vs: seq<pVar>, interp: pInterpretation) 
         returns (result: pInterpretation)
@@ -83,11 +68,8 @@ module truth_table
         var i := | vs | - 1;
         while (i >= 0 ) 
         {
-            // should be able to get rid of this with precondition
             if (! (vs[i] in interp)) { return; }
             assert vs[i] in interp;
-
-            // The first time we find a 0, make it 1 and we're done
             if (interp[ vs[i] ] == false) 
             { 
                 result := result[ vs[i] := true ];
@@ -96,14 +78,15 @@ module truth_table
             else
             {
                 result := result[ vs[i] := false ];
-                // 1 + 1 = 0 plus a carry, so keep looping
             }
-
             i := i - 1;
         }
         return result;
     }
 
+    /*
+    Compute and return 2^n given n.
+    */
     function method pow2(n: nat): (r: nat)
         ensures r >= 1
     { 
