dafny/propositional-logic/variables.dfy
@@ -1,0 +1,93 @@
+include "syntax.dfy"
+
+module variables
+{
+    import opened syntax
+
+        method seqVarsIn(e: pExp) returns (result: seq<pVar>)
+    {
+        /* Compute the set of variables the convert to sequence
+           Dafny does not allow expressions in return statements
+           so we compute and store the results of the expression
+           first, and then return
+        */
+
+        result := setVarsToSeq(getVars(e));
+        return /* result */;
+    }
+
+    /*
+    Given a set of propositional variables, convert it into a 
+    sequence in some arbitrary order by calling a recursive 
+    helper function with an initially empty sequence. This is 
+    a second example of the design pattern seen above.
+
+    Note that Dafny requires the *decreases* statement in the
+    loop specification, to help it know how to prove that the
+    loop terminates. The statement tells Dafny that it is the
+    set, s', that "gets smaller until ulimately bottoming out"
+    at the empty set. 
+    */
+    method setVarsToSeq(s: set<pVar>) returns (result: seq<pVar>)
+    {
+        var l: seq<pVar> := [];
+        var s' := s;
+        while (s' != {}) 
+            decreases s';
+        {
+            var v :| v in s';
+            l := [ v ] + l;
+            s' := s' - { v };
+        }
+        return l;
+    }
+
+/*
+    Given a pExp, we will often need to extract from it
+    the set of variables it uses. This method does that.
+    Note that even if a variable appears multiple times 
+    in an expression it will of course only appear in the
+    set once.
+    */
+    function method getVars(e: pExp): set<pVar>
+    {
+      /*
+      Do the work by calling a recursive helper 
+      function with an empty set as the starting 
+      set to which the variables in the expression
+      will be added.
+      */
+      getVarsHelper(e, {})
+    }
+
+    /*
+    This recursive function adds the set of variables in a 
+    given expression to the set, r, given as an argument. 
+    Note: The getVars and getVarsHelper functions together
+    exhibits a fundamental design pattern called "mutual 
+    recursion". The main function calls the helper function
+    with a partial result to be completed, then the helper
+    function calls the main function recursively to solve
+    sub-parts of the problem it was called to handle. It
+    then combines the results of these subcalls to complete
+    the work it was asked to do.  
+    */
+    function method getVarsHelper(e: pExp, r: set<pVar>): set<pVar>
+    {
+        match e
+        {
+            case pFalse => r
+            case pTrue => r
+            case pVarExp (v: pVar) => r + { v }
+            case pNot (e: pExp) => r + getVars(e)
+            case pAnd (e1: pExp, e2: pExp) =>
+                r + getVars(e1) + getVars(e2)
+            case pOr (e1: pExp, e2: pExp) =>
+                r + getVars(e1) + getVars(e2)
+            case pImpl (e1: pExp, e2: pExp) =>
+                r + getVars(e1) + getVars(e2)
+        }
+    }
+
+ 
+}
